temp_check2.lean
@@ -1,2 +1,5 @@
-import Peano.PeanoNat.ListsAndSets.List
-#check @List.length_erase_of_mem
+import Peano.PeanoNat.Combinatorics.Pow
+open Peano
+#check Peano.Pow.pow_zero
+example (p : ℕ₀) : p ^ 𝟘 = 𝟙 := by
+  exact Peano.Pow.pow_zero p
